TM/Code/Copy.v
@@ -3,6 +3,11 @@
 Require Import TM.Code.CodeTM.
 Require Import TM.Compound.CopySymbols TM.Compound.MoveToSymbol.
 
+Require Import TM.Combinators.Combinators.
+Require Import TM.Basic.Mono.
+Require Import TM.Compound.TMTac.
+Require Import TM.Mirror.
+
 Section Copy.
 
   (*
@@ -55,9 +60,10 @@ Section Copy.
   Lemma CopySymbols_pair_first tltr str1 x str2 tl' tr':
     (forall x, List.In x str1 -> stop x = false) ->
     (stop x = true) ->
-    tape_local (fst tltr) = str1 ++ [x] ++ str2 ->
+    tape_local (fst tltr) = str1 ++ x :: str2 ->
     (tl', tr') = CopySymbols_Fun stop id tltr ->
-    tape_local tl' = x :: str2.
+    tape_local tl' = x :: str2 /\
+    left tl' = rev str1 ++ left (fst tltr).
   Proof.
     intros H H0. destruct tltr as [tl tr]. intros H1 E0.
     destruct tl as [ | r rs | l ls | ls m rs]; cbn in *.
@@ -67,13 +73,13 @@ Section Copy.
     - cbn in *. inv H1. rewrite CopySymbols_Fun_equation in E0. rewrite H0 in E0. inv E0. cbn. auto.
     - rewrite CopySymbols_Fun_equation in E0. destruct (stop m) eqn:E1.
       + inv E0. cbn in *. inv H1. enough (stop s' = false)  by congruence; eauto.
-      + cbn in H1. inv H1. cbn in *. destruct str1'; cbn in *; eapply IHstr1; eauto.
+      + cbn in H1. inv H1. cbn in *. simpl_list. destruct str1'; cbn in *; eapply IHstr1; eauto.
   Qed.
 
   Lemma CopySymbols_pair_second tltr str1 x str2 tl' tr':
     (forall x, List.In x str1 -> stop x = false) ->
     (stop x = true) ->
-    tape_local (fst tltr) = str1 ++ [x] ++ str2 ->
+    tape_local (fst tltr) = str1 ++ x :: str2 ->
     (tl', tr') = CopySymbols_Fun stop id tltr ->
     left tr' = rev str1 ++ left (snd tltr).
   Proof.
@@ -179,3 +185,239 @@ Section Copy.
   Qed.
   
 End Copy.
+
+Section Copy_code.
+  Variable sig : finType.
+  Variable X : Type.
+  Variable encX : codeable sig X.
+
+
+  Variable stop_X : sig -> bool.
+  Hypothesis stop_X_notInX : forall x : X, forall s : sig, List.In s (encode x) -> stop_X s = false.
+
+  Definition stop : (sig^+) -> bool :=
+    fun s => match s with
+          | inl _ => true
+          | inr x => stop_X x
+          end.
+
+  
+  Lemma stop_notInX (x : X) (s : (sig^+)) :
+    List.In s (encode x) -> stop s = false.
+  Proof. cbn. intros (?&<-&?) % in_map_iff. cbn. eapply stop_X_notInX; eauto. Qed.
+
+
+
+  Definition MoveToSymbol_Code := Return (MoveToSymbol stop) tt.
+
+  Definition MoveToSymbol_Code_Rel : Rel (tapes (sig^+) 1) (unit * tapes (sig^+) 1) :=
+    Mono.Mk_R_p (
+        ignoreParam (
+            fun tin tout =>
+              forall (x : X) r1 r2,
+                tape_encodes_l _ tin x r1 r2 ->
+                tape_local_l tout = inl STOP :: rev (encode x) ++ inl START :: r1 /\
+                right tout = r2
+          )
+      ).
+
+
+  
+  (*
+  Definition MoveToSymbol_Code :=
+    MoveToSymbol stop;;
+    MATCH (Read_char _)
+    (fun s => match s with
+           | Some (inl true) => mono_Nop _ tt (* encoding is empty *)
+           | Some (inl false) => Move _ L tt (* encoding is not empty *)
+           | _ => mono_Nop _ tt (* this can't happen *)
+           end).
+   *)
+
+
+  Lemma MoveToSymbol_Code_WRealise :
+    MoveToSymbol_Code ⊫ MoveToSymbol_Code_Rel.
+  Proof.
+    eapply WRealise_monotone.
+    { unfold MoveToSymbol_Code. repeat TM_Correct. }
+    {
+      intros tin ((), tout). TMSimp. clear_trivial_eqs. clear H2.
+      destruct H0 as (HE1&HE2).
+      unfold finType_CS in *.
+      destruct (encode x) eqn:E1.
+      - eapply (MoveToSymbol_correct (stop := stop)) in HE2 as (L1&L2); eauto.
+        split; eauto. cbn in *.
+        + eapply tape_local_cons_iff in L1 as (L1&L1').
+          eapply tape_local_l_cons_iff. split; eauto.
+          rewrite E1. cbn. unfold finType_CS in *. rewrite HE1 in L2. congruence.
+        + eapply tape_local_cons_iff in L1 as (L1&L1'). eauto.
+      - eapply (MoveToSymbol_correct (stop := stop)) in HE2 as (L1&L2); eauto.
+        split; eauto. cbn in *.
+        + eapply tape_local_cons_iff in L1 as (L1&L1').
+          eapply tape_local_l_cons_iff. split; eauto.
+          rewrite E1. cbn. unfold finType_CS in *. rewrite HE1 in L2. congruence.
+        + eapply tape_local_cons_iff in L1 as (L1&L1'). eauto.
+        + intros ? [-> | ?]; eapply (@stop_notInX x); unfold finType_CS in *; rewrite E1; eauto.
+    }
+  Qed.
+
+  Lemma MoveToSymbol_Code_Terminates :
+    projT1 MoveToSymbol_Code ↓
+           (fun tin k => exists x : X, tin[@Fin.F1] ≂ x /\ 4 + 4 * length (encode x) <= k).
+  Proof.
+    eapply TerminatesIn_monotone.
+    { unfold MoveToSymbol_Code. repeat TM_Correct. }
+    {
+      intros tin k. intros (x&HEncX&HTx).
+      destruct HEncX as (r1&r2&HE1&HE2).
+      pose proof MoveToSymbols_TermTime_local (stop := stop) HE2 ltac:(trivial).
+      rewrite <- HTx. progress unfold finType_CS in *. rewrite H.
+      eapply Nat.add_le_mono. omega. cbn. simpl_list. omega.
+    }
+  Qed.
+
+
+
+  Definition MoveToSymbol_Code_L := Return (MoveToSymbol_L stop) tt.
+
+  (*
+  Definition MoveToSymbol_Code_L := Mirror MoveToSymbol_Code.
+
+  Lemma MoveToSymbol_Code_L_WRealise :
+    MoveToSymbol_Code_L ⊫ MoveToSymbol_Code_L_Rel.
+  Proof.
+    eapply WRealise_monotone.
+    { unfold MoveToSymbol_Code_L. repeat TM_Correct. eapply MoveToSymbol_Code_WRealise. }
+    {
+      intros tin (yout, tout) H. hnf in *.
+      intros x r1 r2 (HE1&HE2).
+      specialize (H x r1 r2). spec_assert H.
+      { hnf. simpl_tape. split; auto. 
+
+      specialize H with (1 := HE2).
+    }
+   *)
+
+  Definition MoveToSymbol_Code_L_Rel : Rel (tapes (sig^+) 1) (unit * tapes (sig^+) 1) :=
+    Mono.Mk_R_p (
+        ignoreParam (
+            fun tin tout =>
+              forall (x : X) r1 r2,
+                tape_encodes_r _ tin x r1 r2 ->
+                left tout = r1 /\
+                tape_local tout = inl START :: encode x ++ inl STOP :: r2
+          )
+      ).
+
+    
+  Lemma MoveToSymbol_Code_L_WRealise :
+    MoveToSymbol_Code_L ⊫ MoveToSymbol_Code_L_Rel.
+  Proof.
+    eapply WRealise_monotone.
+    { unfold MoveToSymbol_Code_L. repeat TM_Correct. }
+    {
+      intros tin ((), tout). TMSimp. clear_trivial_eqs. clear H2.
+      destruct H0 as (HE1&HE2).
+      unfold finType_CS in *.
+      destruct (encode x) eqn:E1.
+      - eapply (MoveToSymbol_L_correct (stop := stop)) in HE2 as (L1&L2); eauto.
+        split; eauto. cbn in *.
+        + eapply tape_local_l_cons_iff in L1 as (L1&L1'). eauto.
+        + eapply tape_local_l_cons_iff in L1 as (L1&L1'). unfold finType_CS in *. cbn in *. rewrite E1. cbn.
+          eapply tape_local_cons_iff. split; auto. unfold finType_CS in *. congruence.
+        + cbn. auto.
+      - eapply (MoveToSymbol_L_correct (stop := stop)) in HE2 as (L1&L2); eauto.
+        split; eauto. cbn in *.
+        + eapply tape_local_l_cons_iff in L1 as (L1&L1'). eauto.
+        + eapply tape_local_l_cons_iff in L1 as (L1&L1'). unfold finType_CS in *. cbn in *. rewrite E1. cbn.
+          eapply tape_local_cons_iff. split; auto. unfold finType_CS in *.
+          rewrite rev_app_distr, rev_involutive in L2. cbn in L2. rewrite L2. congruence.
+        + intros ? [ -> | ? ] % in_rev; eapply (@stop_notInX x); unfold finType_CS; rewrite E1; auto.
+    }
+  Qed.
+
+  Lemma MoveToSymbol_Code_L_Terminates :
+    projT1 MoveToSymbol_Code ↓
+           (fun tin k => exists x : X, tin[@Fin.F1] ≂ x /\ 4 + 4 * length (encode x) <= k).
+  Proof.
+    eapply TerminatesIn_monotone.
+    { unfold MoveToSymbol_Code. repeat TM_Correct. }
+    {
+      intros tin k. intros (x&HEncX&HTx).
+      destruct HEncX as (r1&r2&HE1&HE2).
+      pose proof MoveToSymbols_TermTime_local (stop := stop) HE2 ltac:(trivial).
+      rewrite <- HTx. progress unfold finType_CS in *. rewrite H.
+      eapply Nat.add_le_mono. omega. cbn. simpl_list. omega.
+    }
+  Qed.
+
+
+  
+
+
+  Definition CopySymbols_Code := CopySymbols stop id.
+
+  Definition CopySymbols_Code_Rel : Rel (tapes (sig^+) 2) (unit * tapes (sig^+) 2) :=
+    ignoreParam (
+        fun tin tout =>
+          forall x r1 r2,
+            tape_encodes_l _ tin[@Fin.F1] x r1 r2 ->
+            left tout[@Fin.F1] = rev (encode x) ++ inl START :: r1 /\
+            tape_local tout[@Fin.F1] = inl STOP :: r2 /\
+            left tout[@Fin.FS Fin.F1] = rev (encode x) ++ left tin[@Fin.FS Fin.F1]
+      ).
+
+  Lemma CopySymbols_Code_WRealise :
+    CopySymbols_Code ⊫ CopySymbols_Code_Rel.
+  Proof.
+    eapply WRealise_monotone.
+    { unfold CopySymbols_Code. repeat TM_Correct. }
+    {
+      intros tin ((), tout). TMSimp. clear_trivial_eqs.
+      destruct H0 as (HE1&HE2).
+      destruct (encode x) eqn:E1.
+      - unshelve epose proof CopySymbols_pair_first (stop := stop) as L.
+        specialize L with (4 := H). cbn in L. specialize L with (3 := HE2).
+        spec_assert L by eauto. spec_assert L as (L1&L2) by eauto.
+
+        unshelve epose proof CopySymbols_pair_second (stop := stop) as L.
+        specialize L with (4 := H). cbn in L. specialize L with (3 := HE2).
+        spec_assert L by eauto. spec_assert L by eauto.
+        cbn in *. rewrite E1 in *. cbn. split; auto.
+        rewrite HE1 in *. auto.
+      - unshelve epose proof CopySymbols_pair_first (stop := stop) as L.
+        specialize L with (4 := H). cbn in L. specialize L with (3 := HE2).
+        spec_assert L.
+        { intros ? [-> | ?]; eapply (@stop_notInX x); unfold finType_CS in *; rewrite E1; eauto. }
+        spec_assert L as (L1&L2) by eauto.
+
+        unshelve epose proof CopySymbols_pair_second (stop := stop) as L.
+        specialize L with (4 := H). cbn in L. specialize L with (3 := HE2).
+        spec_assert L.
+        { intros ? [-> | ?]; eapply (@stop_notInX x); unfold finType_CS in *; rewrite E1; eauto. }
+        spec_assert L by eauto.
+        cbn in *. rewrite E1 in *. cbn. split; auto.
+        rewrite HE1 in *. auto.
+    }
+  Qed.
+
+  (* TODO: Termination *)
+
+  (* TODO: Gespiegelte Variante *)
+                 
+End Copy_code.
+
+Arguments MoveToSymbol_Code : simpl never.
+Arguments CopySymbols_Code : simpl never.
+
+Arguments MoveToSymbol_Code_Rel { sig X encX } x y /.
+Arguments CopySymbols_Code_Rel { sig X encX } x y /.
+
+Ltac smpl_TM_CopyMoveCode :=
+  match goal with
+  | [ |- MoveToSymbol_Code    _ ⊫ _ ] => eapply MoveToSymbol_Code_WRealise
+  | [ |- MoveToSymbol_Code_L  _ ⊫ _ ] => eapply MoveToSymbol_Code_L_WRealise
+  | [ |- CopySymbols_Code     _ ⊫ _ ] => eapply CopySymbols_Code_WRealise
+  end.
+
+Smpl Add smpl_TM_CopyMoveCode : TM_Correct.
